$
(a+b)^{2} 
\\ = (a+b)\cdot(a+b)
\\ = a \cdot (a+b) + b \cdot (a+b)
\\ = a \cdot a + a \cdot b + b \cdot a + b \cdot b
\\ = a ^ {2} + a\cdot b + a \cdot b+ b ^ {2} 
\\ = a ^ {2} + 2a\cdot b + b ^ {2} 
$

$
(a-b)^{2} 
\\ = (a-b)\cdot(a-b)
\\ = a \cdot (a-b) - b \cdot (a-b)
\\ = a \cdot a - a \cdot b - b \cdot a + b \cdot b
\\ = a ^ {2} - a\cdot b - a \cdot b+ b ^ {2} 
\\ = a ^ {2} - 2a\cdot b + b ^ {2} 
$


$
S_{ABDE} 
\\ = c^2
\\ = S_{ACB} + S_{BHD} + S_{DFE} + S_{EGA} + S_{CHFG}
\\ = 4(\frac{1}{2} \cdot ab) + (b-a)^2 
\\ = 2ab + (b-a)^2
\\ = 2ab + b^2 + a ^2 - 2ab
= a^2 + b^2
$

$
S_{ABCD} 
\\ = (a+b)^2
\\ = S_{AEFG} + S_{EBIF} + S_{ICHF} + S_{FGDH}
\\ = a^2 + ab + b^2 + ab
\\ = a^2 + 2ab + b^2
$


$
S_{ABCD} 
\\ = a^2
\\ = S_{AEFG} + S_{EBCJ} + S_{DGHC} - S_{FHCJ}
\\ = (a-b)^2 + ab + ab - b^2
\\ = (a-b)^2 + 2ab - b^2
\\
\iff
\\ 
a^2 - 2ab + b^2
\\ = (a-b)^2 
\\
\iff
\\ 
(a-b)^2 
\\ =  a^2 - 2ab + b^2
$

$
S_{ABC} = \frac{1}{2} \overline{AB} \cdot  \overline{BC}
\\ = S_{ABE} + S_{CBE}
\\ = \frac{1}{2} \overline{AE} \cdot  \overline{EB} + \frac{1}{2} \overline{EC} \cdot  \overline{EB}
\\ = \frac{1}{2} (\overline{AE} + \overline{EC}) \cdot  \overline{EB}
\\ = \frac{1}{2} \overline{AC} \cdot  \overline{EB}
$


$
S_{ABC} = \frac{1}{2} \overline{AB} \cdot  \overline{BC}
\\ = S_{ABE} + S_{CBE}
\\ = \frac{1}{2} \overline{AE} \cdot  \overline{EB} + \frac{1}{2} \overline{EC} \cdot  \overline{EB}
\\ = \frac{1}{2} (\overline{AE} + \overline{EC}) \cdot  \overline{EB}
\\ = \frac{1}{2} \overline{AC} \cdot  \overline{EB}
$

$
\triangle ABC 和 \triangle A_{1}B_{1}C_{1}
\\ AB = A_{1}B_{1}
\\ \angle{ABC} = \angle{A_{1}B_{1}C_{1}}
\\ BC = B_{1}C_{1}
\\ \Rightarrow
\\ ABC \cong A_{1}B_{1}C_{1}
$


$
\triangle ABC 和 \triangle A_{1}B_{1}C_{1}
\\ \angle{CAB} = \angle{C_{1}A_{1}B_{1}}
\\ AB = A_{1}B_{1}
\\ \angle{CBA} = \angle{C_{1}B_{1}A_{1}}
\\ \Rightarrow
\\ ABC \cong A_{1}B_{1}C_{1}
$